Classical_Grounding/Planner_Export.thy
@@ -20,6 +20,9 @@ text \<open>\<^bold>\<open>The default SML export of the session\<close> (the on
 export_code
   plan_by_cert_dfs ground_via_cert'_dfs ground_via_cert_dfs
   ground_via_cert_numeric_dfs_e ground_via_cert_numeric_exec_e ground_via_cert_numeric_gdfs_e
+  ground_via_cert_numeric_dfs_stream_e ground_via_cert_numeric_exec_stream_e ground_via_cert_numeric_gdfs_stream_e
+  ast_classical_problem.P\<^sub>T cert_ops_of_exec_fast canon ast_classical_problem.numeric_ground_ac
+  distinct_strings_lit
   ground_via_cert_prop_dfs_e
   dl_program_of sat_solve_strips
   reconstruct_plan_by_cert reconstruct_plan_by_cert_numeric
